Splinter/BranchTreeInterp.i.dfy
@@ -12,7 +12,7 @@ include "../lib/Base/mathematics.i.dfy"
 module BranchTreeInterpMod {
   import opened Options
   import opened ValueMessage
-  import KeyType
+  import opened KeyType
   import opened InterpMod
   import opened DiskTypesMod
   import opened AllocationMod
@@ -25,7 +25,6 @@ module BranchTreeInterpMod {
 
   type Lookup = BranchPath
 
-  //function IMLookup()
 
   // NOtE: These might not be needed.
   function IMKey(root: CU, cache: CacheIfc.Variables, key: Key) : Message
@@ -48,9 +47,47 @@ module BranchTreeInterpMod {
     imap k | true :: IMKey(root, cache, k)
   }
 
-  function IReadsKey(v: Variables, cache: CacheIfc.Variables, key: Key) : set<CU>
+  predicate ValidLookupHasCU(cache: CacheIfc.Variables, lookup: BranchPath, cu: CU)
+  {
+    && lookup.Valid(cache)
+    && cu in lookup.CUs()
+  }
 
-  function IReads(v: Variables, cache: CacheIfc.Variables) : set<CU>
+  // IREAds lookup
+  function {:opaque} IReadsLookup(cache: CacheIfc.Variables, lookup: BranchPath) : set<CU> {
+    set cu:CU |
+       && cu in CUsInDisk()
+       && ValidLookupHasCU(cache, lookup, cu)
+      :: cu
+  }
+
+  predicate StepsEquivalent(cache0: CacheIfc.Variables, cache1: CacheIfc.Variables, step0: BranchStep, step1: BranchStep)
+  {
+    //&& step0.cu == step1.cu
+    && step0.Valid(cache0)
+    && step1.Valid(cache1)
+    && step0.cu == step1.cu
+    && CUToBranchNode(step0.cu, cache0) == CUToBranchNode(step1.cu, cache1)
+  }
+
+  predicate StepsLinked(cache: CacheIfc.Variables, lookup: BranchPath, currStep: nat, currStepCU: CU, nextStepCU : CU)
+    requires currStep < |lookup.steps| - 1
+  {
+    // make sure cus match with the ones in the branchpath
+    && currStepCU == lookup.steps[currStep].cu
+    && nextStepCU == lookup.steps[currStep+1].cu
+    // The lookup has to be valid
+    && lookup.Valid(cache)
+    // make sure there's a valid link at the lookup -- Might not be needed, we might be getting this from Valid(s)
+    && lookup.LinkedAt(currStep+1)
+    // Check if these loose steps correspond to parent-child
+    && var currNode := CUToBranchNode(currStepCU, cache);
+    && var nextNode := CUToBranchNode(nextStepCU, cache);
+    && currNode.Some?
+    && nextNode.Some?
+    && currNode.value == lookup.steps[currStep].node
+    && nextNode.value == lookup.steps[currStep+1].node
+  }
 
   lemma BranchLookupsEquivalentInductive(v: Variables,
                                 cache0: CacheIfc.Variables,
@@ -61,32 +98,79 @@ module BranchTreeInterpMod {
     requires lookup0.key == lookup1.key
     requires lookup0.Valid(cache0)
     requires lookup1.Valid(cache1)
+    requires 0 < count
     requires count <= |lookup0.steps|
     requires count <= |lookup1.steps|
-    requires DiskViewsEquivalent(cache0.dv, cache1.dv, IReads(v, cache0))
-    ensures forall i :: ((0 <= i < count) ==> (lookup0.steps[i] == lookup1.steps[i]))
+    //requires lookup0.steps[0].cu == lookup1.steps[0].cu
+    requires DiskViewsEquivalent(cache0.dv, cache1.dv, IReadsLookup(cache0, lookup0))
+    requires DiskViewsEquivalent(cache1.dv, cache1.dv, IReadsLookup(cache1, lookup1))
+    ensures forall i :: ((0 < i < count-1) ==>  && StepsLinked(cache0, lookup0, i, lookup0.steps[i].cu, lookup0.steps[i+1].cu)
+                                                && StepsLinked(cache1, lookup1, i, lookup1.steps[i].cu, lookup1.steps[i+1].cu))
+    ensures forall i :: ((0 <= i < count) ==> StepsEquivalent(cache0, cache1, lookup0.steps[i], lookup1.steps[i]))
     {
-      if count == 0 {
+      if 1 < count {
+        BranchLookupsEquivalentInductive(v, cache0, cache1, lookup0, lookup1, count - 1);
+        var step0 :=  lookup0.steps[count-2];
+        var step1 :=  lookup1.steps[count-2];
+
+        //assert step0.cu in IReadsLookup(cache0, lookup0);
+        //assert step1.cu in IReadsLookup(cache0, lookup0);
+
+        assert step0.cu == step1.cu; // All we need to show is that the CUs are the same
+        assert CUToBranchNode(step0.cu, cache0) == CUToBranchNode(step1.cu, cache1);
+
+        // route to next node
+        var nextStep0 := lookup0.steps[count-1];
+        var nextStep1 := lookup1.steps[count-1];
+
+        assert StepsEquivalent(cache0, cache1, step0, step1);
+        assert StepsEquivalent(cache0, cache1, nextStep0, nextStep1);
+        assert StepsLinked(cache0, lookup0, count-1, step0.cu, nextStep0.cu);
+        assert StepsLinked(cache1, lookup1, count-1, step1.cu, nextStep1.cu);
 
       } else {
-        BranchLookupsEquivalentInductive(v, cache0, cache1, lookup0, lookup1, count - 1);
-        var step0 :=  lookup0.steps[count-1];
-        var step1 :=  lookup1.steps[count-1];
+        assert count == 1;
       }
     }
 
+    predicate ValidLookupForBranchEquivalent(cache0: CacheIfc.Variables,
+                                             cache1: CacheIfc.Variables,
+                                             receipt0: BranchReceipt,
+                                             receipt1: BranchReceipt)
+    {
+      && var lookup0 := receipt0.branchPath;
+      && var lookup1 := receipt1.branchPath;
+      && lookup0.key == lookup1.key
+      && lookup0.Valid(cache0)
+      && lookup1.Valid(cache1)
+    }
+
+    predicate RootEquivalentForBranchReceipts(cache0: CacheIfc.Variables,
+                                              cache1: CacheIfc.Variables,
+                                              receipt0: BranchReceipt,
+                                              receipt1: BranchReceipt)
+    {
+      && receipt0.Valid(cache0)
+      && receipt1.Valid(cache1)
+      && var cu0 := receipt0.branchTree.Root();
+      && var cu1 := receipt1.branchTree.Root();
+      && cu0 == cu1
+      && CacheIfc.ReadValue(cache0, cu0) == CacheIfc.ReadValue(cache1, cu1)
+    }
 
     lemma BranchLookupsEquivalent(v: Variables,
                                   cache0: CacheIfc.Variables,
                                   cache1: CacheIfc.Variables,
-                                  lookup0: BranchPath,
-                                  lookup1: BranchPath)
-      requires lookup0.key == lookup1.key
-      requires lookup0.Valid(cache0)
-      requires lookup1.Valid(cache1)
-      requires DiskViewsEquivalent(cache0.dv, cache1.dv, IReads(v, cache0))
-      ensures  lookup0 == lookup1
+                                  receipt0: BranchReceipt,
+                                  receipt1: BranchReceipt)
+
+      requires ValidLookupForBranchEquivalent(cache0, cache1, receipt0, receipt1)
+      requires RootEquivalentForBranchReceipts(cache0, cache1, receipt0, receipt1)
+      requires DiskViewsEquivalent(cache0.dv, cache1.dv, IReadsLookup(cache0, receipt0.branchPath))
+      ensures  receipt0 == receipt1
       {
+        var lookup0 := receipt0.branchPath;
+        var lookup1 := receipt1.branchPath;
         var minLookup := min(|lookup0.steps|, |lookup1.steps|);
         BranchLookupsEquivalentInductive(v, cache0, cache1, lookup0, lookup1, minLookup);
       }
